Defined a coinductive divergence based on well-formedness, and proved that it equals to the other two versions of divergence. This finished the top-level simulation proofs of phinode-placement.
NOTE: In a coinductive constructor, Coq does not allow to use an inductive 
proof that uses the coinductive hypothesis because of its syntax
restriction. For such proofs, we should swap the inductive proofs and
and the coinductive hypothesis to let coinductive constructors see the
nested coinductive hyp directly, which is checked by Coq.



git-svn-id: https://webdav.seas.upenn.edu/svn/sol/vol@3782 eef5ea85-cc2e-0410-bd84-0fae1f012da8

src3.0/Transforms/phiplacement_bsim.v
@@ -21,6 +21,165 @@ Import Promotability.
 
 Definition DGVMap := @Opsem.GVsMap DGVs.
 
+Lemma sop_plus_star__implies__sop_plus: forall cfg S1 S2 S3 tr1 tr2,
+  Opsem.sop_plus cfg S1 S2 tr1 ->
+  @Opsem.sop_star DGVs cfg S2 S3 tr2 ->
+  Opsem.sop_plus cfg S1 S3 (tr1 ** tr2).
+Proof.
+  induction 1; intros; auto.
+    rewrite Eapp_assoc; auto. 
+    econstructor; eauto.
+    eapply OpsemProps.sop_star_trans; eauto.
+Qed.
+
+Lemma sop_star_plus__implies__sop_plus: forall cfg S1 S2 S3 tr1 tr2,
+  @Opsem.sop_star DGVs cfg S1 S2 tr1 ->
+  Opsem.sop_plus cfg S2 S3 tr2 ->
+  Opsem.sop_plus cfg S1 S3 (tr1 ** tr2).
+Proof.
+  induction 1; intros; auto.
+    apply IHsop_star in H1.
+    rewrite Eapp_assoc; auto. 
+    econstructor; eauto.
+    eapply OpsemProps.sop_plus__implies__sop_star; eauto.
+Qed.
+
+Lemma sop_step_plus__implies__sop_plus: forall cfg S1 S2 S3 tr1 tr2,
+  Opsem.sInsn cfg S1 S2 tr1 ->
+  @Opsem.sop_plus DGVs cfg S2 S3 tr2 ->
+  Opsem.sop_plus cfg S1 S3 (tr1 ** tr2).
+Proof.
+  intros. inv H0.
+  econstructor; eauto.
+Qed.
+
+CoInductive sop_diverges' (cfg:OpsemAux.Config): 
+    @Opsem.State DGVs -> traceinf -> Prop :=
+| sop_diverges_intro' : forall state1 state2 tr1 tr2,
+    Opsem.sInsn cfg state1 state2 tr1 ->
+    sop_diverges' cfg state2 tr2 ->
+    sop_diverges' cfg state1 (Eappinf tr1 tr2).
+
+Lemma sop_star_diverges'__sop_diverges': forall cfg IS1 IS2 tr1 tr2,
+  Opsem.sop_star cfg IS1 IS2 tr1 ->
+  sop_diverges' cfg IS2 tr2 ->
+  sop_diverges' cfg IS1 (Eappinf tr1 tr2).
+Proof.
+  induction 1; intros; auto.
+    apply IHsop_star in H1.
+    rewrite Eappinf_assoc.
+    econstructor; eauto.
+Qed.
+
+Lemma sop_plus_diverges'__sop_diverges': forall cfg IS1 IS2 tr1 tr2,
+  Opsem.sop_plus cfg IS1 IS2 tr1 ->
+  sop_diverges' cfg IS2 tr2 ->
+  sop_diverges' cfg IS1 (Eappinf tr1 tr2).
+Proof.
+  intros. inv H.
+  eapply sop_star_diverges'__sop_diverges' in H2; eauto.
+  rewrite Eappinf_assoc.
+  econstructor; eauto.
+Qed.
+
+Lemma sop_star_diverges__sop_diverges: forall cfg IS1 IS2 tr1 tr2,
+  @Opsem.sop_star DGVs cfg IS1 IS2 tr1 ->
+  Opsem.sop_diverges cfg IS2 tr2 ->
+  Opsem.sop_diverges cfg IS1 (Eappinf tr1 tr2).
+Proof.
+  induction 1; intros; auto.
+    apply IHsop_star in H1.
+    rewrite Eappinf_assoc.
+    rewrite <- E0_right at 1.
+    econstructor; eauto.
+Qed.
+
+Lemma sop_diverges__sop_diverges': forall cfg IS tr,
+  @Opsem.sop_diverges DGVs cfg IS tr -> sop_diverges' cfg IS tr.
+Proof.
+  cofix CIH.
+  intros.
+  inv H.
+  inv H0.
+  assert (Opsem.sop_diverges cfg state0 (tr3***tr2)) as J.
+    clear CIH. 
+    eapply sop_star_diverges__sop_diverges; eauto.
+  apply CIH in J. clear CIH.
+  rewrite Eappinf_assoc.
+  econstructor; eauto.
+Qed.
+
+Lemma sop_diverges'__sop_diverges: forall cfg IS tr,
+  sop_diverges' cfg IS tr -> @Opsem.sop_diverges DGVs cfg IS tr.
+Proof.
+  cofix CIH.
+  intros.
+  inv H.
+  apply CIH in H1. clear CIH.
+  econstructor; eauto.
+    rewrite <- E0_right.
+    econstructor; eauto.
+Qed.
+
+Section SOP_WF_DIVERGES.
+
+Variable Measure: Type.
+Variable R:Measure -> Measure -> Prop.
+Hypothesis Hwf_founded_R: well_founded R.
+
+CoInductive sop_wf_diverges (cfg:OpsemAux.Config): 
+    Measure -> @Opsem.State DGVs -> traceinf -> Prop :=
+| sop_wf_diverges_plus : forall m1 m2 state1 state2 tr1 tr2,
+    Opsem.sop_plus cfg state1 state2 tr1 ->
+    sop_wf_diverges cfg m2 state2 tr2 ->
+    sop_wf_diverges cfg m1 state1 (Eappinf tr1 tr2)
+| sop_wf_diverges_star : forall m1 m2 state1 state2 tr1 tr2,
+    R m2 m1 ->
+    Opsem.sop_star cfg state1 state2 tr1 ->
+    sop_wf_diverges cfg m2 state2 tr2 ->
+    sop_wf_diverges cfg m1 state1 (Eappinf tr1 tr2)
+.
+
+Lemma sop_wf_diverges__inv: forall m1 cfg S1 Tr
+  (Hdiv: sop_wf_diverges cfg m1 S1 Tr),
+  exists S2, exists m2, exists tr, exists Tr',
+    Opsem.sop_plus cfg S1 S2 tr /\
+    sop_wf_diverges cfg m2 S2 Tr' /\
+    Tr = Eappinf tr Tr'.
+Proof.
+  intro m1. pattern m1.
+  apply (well_founded_ind Hwf_founded_R); intros.
+  inv Hdiv.
+    exists state2. exists m2. exists tr1. exists tr2. 
+    split; auto.
+
+    apply H in H2; auto.
+    destruct H2 as [S2 [m2' [tr [Tr' [J1 [J2 J3]]]]]]; subst.
+    exists S2. exists m2'. exists (Eapp tr1 tr). exists Tr'.
+    split.
+      eapply sop_star_plus__implies__sop_plus; eauto.
+    split; auto.
+      rewrite Eappinf_assoc; auto.
+Qed.
+
+Lemma sop_wf_diverges__sop_diverges: forall cfg m IS tr,
+  sop_wf_diverges cfg m IS tr -> Opsem.sop_diverges cfg IS tr.
+Proof.
+  cofix CIH.
+  intros.
+  inv H.
+    apply sop_wf_diverges__inv in H1; auto.
+    destruct H1 as [S2 [m2' [tr [Tr' [J1 [J2 J3]]]]]]; subst.
+    econstructor; eauto.
+
+    apply sop_wf_diverges__inv in H2; auto.
+    destruct H2 as [S2 [m2' [tr [Tr' [J1 [J2 J3]]]]]]; subst.
+    rewrite <- Eappinf_assoc.
+    econstructor; eauto using sop_star_plus__implies__sop_plus.
+Qed.
+
+End SOP_WF_DIVERGES.
+
 Definition reg_simulation (pinfo: PhiInfo) (f1:fdef) (lc1 lc2:DGVMap) : Prop :=  
   if (fdef_dec (PI_f pinfo) f1) then 
     (forall i0, 
@@ -1876,7 +2035,7 @@ Lemma phinodes_placement_is_correct__dsBranch: forall
   (H2 : Opsem.switchToNewBasicBlock TD (block_intro l' ps' cs' tmn') B gl lc =
        ret lc'),
   exists St1' : Opsem.State,
-     Opsem.sop_star Cfg1 St1 St1' E0 /\
+     Opsem.sop_plus Cfg1 St1 St1' E0 /\
      State_simulation pinfo Cfg1 St1' Cfg2
      {|Opsem.ECS := {| Opsem.CurFunction := F;
                        Opsem.CurBB := (block_intro l' ps' cs' tmn');
@@ -2028,7 +2187,7 @@ Proof.
                 lc1' als)::ECs1) Mem).
     split.
     SSCase "opsem".
-      apply OpsemProps.sInsn__implies__sop_star.
+      apply OpsemProps.sInsn__implies__sop_plus.
       econstructor; eauto.
 
     SSCase "sim".
@@ -2066,7 +2225,7 @@ Proof.
               ::ECs1) Mem).
     split.
     SSCase "opsem".
-      apply OpsemProps.sInsn__implies__sop_star.
+      apply OpsemProps.sInsn__implies__sop_plus.
       econstructor; eauto.
 
     SSCase "sim".
@@ -2112,7 +2271,7 @@ Lemma phinodes_placement_is_correct__dsBranch_uncond: forall
   (H2 : Opsem.switchToNewBasicBlock TD (block_intro l' ps' cs' tmn') B gl lc =
        ret lc'),
   exists St1' : Opsem.State,
-     Opsem.sop_star Cfg1 St1 St1' E0 /\
+     Opsem.sop_plus Cfg1 St1 St1' E0 /\
      State_simulation pinfo Cfg1 St1' Cfg2
      {|Opsem.ECS := {| Opsem.CurFunction := F;
                        Opsem.CurBB := (block_intro l' ps' cs' tmn');
@@ -2248,7 +2407,7 @@ Proof.
               lc1' als)::ECs1) Mem).
     split.
     SSCase "opsem".
-      apply OpsemProps.sInsn__implies__sop_star.
+      apply OpsemProps.sInsn__implies__sop_plus.
       econstructor; eauto.
 
     SSCase "sim".
@@ -2286,7 +2445,7 @@ Proof.
               ::ECs1) Mem).
     split.
     SSCase "opsem".
-      apply OpsemProps.sInsn__implies__sop_star.
+      apply OpsemProps.sInsn__implies__sop_plus.
       econstructor; eauto.
 
     SSCase "sim".
@@ -2450,6 +2609,12 @@ Proof.
       eapply wf_tmp_value__updateAddAL_neq; eauto.
 Qed.
 
+Definition measure (st:@Opsem.State DGVs) : nat :=
+match st with 
+| {| Opsem.ECS := {| Opsem.CurCmds := cs |} :: _ |} => List.length cs
+| _ => 0%nat
+end.
+
 Lemma phinodes_placement_is_correct__dsLoad: forall (maxb : Values.block) 
   (pinfo : PhiInfo)
   (Cfg1 : OpsemAux.Config) (St1 : Opsem.State) (Hwfpi : WF_PhiInfo pinfo)
@@ -2476,8 +2641,8 @@ Lemma phinodes_placement_is_correct__dsLoad: forall (maxb : Values.block)
   (mps : GVsT DGVs) (mp : GenericValue) (gv : GenericValue)
   (H : Opsem.getOperandValue TD v lc gl = ret mps)
   (H0 : mp @ mps) (H1 : mload TD Mem mp t align0 = ret gv),
-  exists St1' : Opsem.State,
-     Opsem.sop_star Cfg1 St1 St1' E0 /\
+  (exists St1' : Opsem.State,
+     Opsem.sop_plus Cfg1 St1 St1' E0 /\
      State_simulation pinfo Cfg1 St1' Cfg2
        {|
        Opsem.ECS := {|
@@ -2488,7 +2653,37 @@ Lemma phinodes_placement_is_correct__dsLoad: forall (maxb : Values.block)
                     Opsem.Locals := updateAddAL (GVsT DGVs) lc id0
                                       ($ gv # t $);
                     Opsem.Allocas := als |} :: EC;
-       Opsem.Mem := Mem |}.
+       Opsem.Mem := Mem |}) \/
+  (exists St1' : Opsem.State,
+     Opsem.sop_star Cfg1 St1 St1' E0 /\
+     lt (measure ({| Opsem.ECS := {|
+                          Opsem.CurFunction := F;
+                          Opsem.CurBB := B;
+                          Opsem.CurCmds := cs;
+                          Opsem.Terminator := tmn;
+                          Opsem.Locals := updateAddAL (GVsT DGVs) lc id0
+                                              ($ gv # t $);
+                          Opsem.Allocas := als |} :: EC;
+                     Opsem.Mem := Mem |}))
+        (measure ({| Opsem.ECS := {|
+                          Opsem.CurFunction := F;
+                          Opsem.CurBB := B;
+                          Opsem.CurCmds := insn_load id0 t v align0 :: cs;
+                          Opsem.Terminator := tmn;
+                          Opsem.Locals := lc;
+                          Opsem.Allocas := als |} :: EC;
+                     Opsem.Mem := Mem |})) /\
+     State_simulation pinfo Cfg1 St1' Cfg2
+       {|
+       Opsem.ECS := {|
+                    Opsem.CurFunction := F;
+                    Opsem.CurBB := B;
+                    Opsem.CurCmds := cs;
+                    Opsem.Terminator := tmn;
+                    Opsem.Locals := updateAddAL (GVsT DGVs) lc id0
+                                      ($ gv # t $);
+                    Opsem.Allocas := als |} :: EC;
+       Opsem.Mem := Mem |}).
 Proof.
   intros. subst.
   destruct_ctx_other.
@@ -2506,6 +2701,7 @@ Proof.
         subst.
       inv J2.
 
+      right.
       exists 
         {| Opsem.ECS := {|
                     Opsem.CurFunction := PI_f pinfo;
@@ -2514,10 +2710,11 @@ Proof.
                     Opsem.Terminator := tmn;
                     Opsem.Locals := lc1;
                     Opsem.Allocas := als |} :: ECs1;
-           Opsem.Mem := Mem |}.
+           Opsem.Mem := Mem |}. simpl.
       split.
       SSCase "opsem".
         constructor.
+      split; auto.
       SSCase "sim".
         repeat (split; eauto 2 using cmds_at_block_tail_next).
 
@@ -2571,6 +2768,7 @@ Proof.
     SCase "isnt_temporary".
       apply cmds_simulation_same_cons_inv in Htcmds; eauto.
       destruct Htcmds as [cs1' [Heq Htcmds]]; subst.
+      left.
       exists 
         (Opsem.mkState 
           ((Opsem.mkEC (PI_f pinfo) 
@@ -2579,7 +2777,7 @@ Proof.
          ::ECs1) Mem).
       split.
       SSCase "opsem".
-        apply OpsemProps.sInsn__implies__sop_star.
+        apply OpsemProps.sInsn__implies__sop_plus.
         econstructor; eauto.
           erewrite simulation__getOperandValue; eauto.
             eapply original_values_in_cmd_arent_tmps; eauto; simpl; auto.
@@ -2593,6 +2791,7 @@ Proof.
   Case "PI_f pinfo <> F1".
     apply cmds_simulation_other_cons_inv in Htcmds; auto.
     destruct Htcmds as [cs1' [Heq Htcmds]]; subst.
+    left.
     exists 
       (Opsem.mkState 
         ((Opsem.mkEC F1
@@ -2601,7 +2800,7 @@ Proof.
        ::ECs1) Mem).
     split.
     SSCase "opsem".
-      apply OpsemProps.sInsn__implies__sop_star.
+      apply OpsemProps.sInsn__implies__sop_plus.
       econstructor; eauto.
         erewrite simulation__getOperandValue; eauto.
           eapply original_values_in_cmd_arent_tmps; eauto; simpl; auto.
@@ -2705,8 +2904,8 @@ Lemma phinodes_placement_is_correct__dsStore: forall (maxb : Values.block)
   (mps2 : GVsT DGVs) (H : Opsem.getOperandValue TD v1 lc gl = ret gvs1)
   (H0 : Opsem.getOperandValue TD v2 lc gl = ret mps2) (H1 : gv1 @ gvs1)
   (H2 : mp2 @ mps2) (H3 : mstore TD Mem mp2 t gv1 align0 = ret Mem'),
-  exists St1' : Opsem.State,
-     Opsem.sop_star Cfg1 St1 St1' E0 /\
+  (exists St1' : Opsem.State,
+     Opsem.sop_plus Cfg1 St1 St1' E0 /\
      State_simulation pinfo Cfg1 St1' Cfg2
        {|
        Opsem.ECS := {|
@@ -2716,7 +2915,35 @@ Lemma phinodes_placement_is_correct__dsStore: forall (maxb : Values.block)
                     Opsem.Terminator := tmn;
                     Opsem.Locals := lc;
                     Opsem.Allocas := als |} :: EC;
-       Opsem.Mem := Mem' |}.
+       Opsem.Mem := Mem' |}) \/
+  (exists St1' : Opsem.State,
+     Opsem.sop_star Cfg1 St1 St1' E0 /\
+     lt (measure ({| Opsem.ECS := {|
+                          Opsem.CurFunction := F;
+                          Opsem.CurBB := B;
+                          Opsem.CurCmds := cs;
+                          Opsem.Terminator := tmn;
+                          Opsem.Locals := lc;
+                          Opsem.Allocas := als |} :: EC;
+                     Opsem.Mem := Mem' |}))
+        (measure ({| Opsem.ECS := {|
+                          Opsem.CurFunction := F;
+                          Opsem.CurBB := B;
+                          Opsem.CurCmds := insn_store sid t v1 v2 align0 :: cs;
+                          Opsem.Terminator := tmn;
+                          Opsem.Locals := lc;
+                          Opsem.Allocas := als |} :: EC;
+                     Opsem.Mem := Mem |})) /\
+     State_simulation pinfo Cfg1 St1' Cfg2
+       {|
+       Opsem.ECS := {|
+                    Opsem.CurFunction := F;
+                    Opsem.CurBB := B;
+                    Opsem.CurCmds := cs;
+                    Opsem.Terminator := tmn;
+                    Opsem.Locals := lc;
+                    Opsem.Allocas := als |} :: EC;
+       Opsem.Mem := Mem' |}).
 Proof.
   intros. subst.
   destruct_ctx_other.
@@ -2734,6 +2961,7 @@ Proof.
                            [J1 [J2 [J3 J4]]]]]]]]]]]; subst.
       inv J1. inversion Heq1; subst l1 ps1 tmn.
       apply app_inv_tail_nil in H8; subst. simpl.
+      right.
       exists 
         {| Opsem.ECS := {|
                     Opsem.CurFunction := PI_f pinfo;
@@ -2742,10 +2970,11 @@ Proof.
                     Opsem.Terminator := tmn1;
                     Opsem.Locals := lc1;
                     Opsem.Allocas := als |} :: ECs1;
-           Opsem.Mem := Mem |}.
+           Opsem.Mem := Mem |}. simpl.
       split.
       SSCase "opsem".
         constructor.
+      split; auto.
       SSCase "sim".
         repeat (split; eauto 2 using cmds_at_block_tail_next).
 
@@ -2810,6 +3039,7 @@ Proof.
     SCase "isnt_temporary".
       apply cmds_simulation_same_cons_inv in Htcmds; eauto.
       destruct Htcmds as [cs1' [Heq Htcmds]]; subst.
+      left.
       exists 
         (Opsem.mkState 
           ((Opsem.mkEC (PI_f pinfo) 
@@ -2819,7 +3049,7 @@ Proof.
          ::ECs1) Mem').
       split.
       SSCase "opsem".
-        apply OpsemProps.sInsn__implies__sop_star.
+        apply OpsemProps.sInsn__implies__sop_plus.
         erewrite <- simulation__getOperandValue in H; eauto.
         erewrite <- simulation__getOperandValue in H0; eauto.
         eapply original_values_in_cmd_arent_tmps; eauto; simpl; auto.
@@ -2836,6 +3066,7 @@ Proof.
   Case "PI_f pinfo <> F1".
       apply cmds_simulation_other_cons_inv in Htcmds; eauto.
       destruct Htcmds as [cs1' [Heq Htcmds]]; subst.
+      left.
       exists 
         (Opsem.mkState 
           ((Opsem.mkEC F1
@@ -2845,7 +3076,7 @@ Proof.
          ::ECs1) Mem').
       split.
       SSCase "opsem".
-        apply OpsemProps.sInsn__implies__sop_star.
+        apply OpsemProps.sInsn__implies__sop_plus.
         erewrite <- simulation__getOperandValue in H; eauto.
         erewrite <- simulation__getOperandValue in H0; eauto.
         eapply original_values_in_cmd_arent_tmps; eauto; simpl; auto.
@@ -2863,7 +3094,7 @@ Ltac next_state :=
 match goal with
 | Hrsim: reg_simulation ?pinfo ?F1 ?lc1 ?lc |-
      exists St1' : Opsem.State,
-     Opsem.sop_star _
+     Opsem.sop_plus _
        {|
        Opsem.ECS := {|
                     Opsem.CurFunction := ?F1;
@@ -2890,7 +3121,7 @@ match goal with
 
 | Hrsim: reg_simulation ?pinfo ?F1 ?lc1 ?lc |-
      exists St1' : Opsem.State,
-     Opsem.sop_star _
+     Opsem.sop_plus _
        {|
        Opsem.ECS := {|
                     Opsem.CurFunction := ?F1;
@@ -2918,7 +3149,7 @@ match goal with
 
 | Hrsim: reg_simulation ?pinfo ?F1 ?lc1 ?lc |-
      exists St1' : Opsem.State,
-     Opsem.sop_star _
+     Opsem.sop_plus _
        {|
        Opsem.ECS := {|
                     Opsem.CurFunction := ?F1;
@@ -3003,7 +3234,7 @@ match goal with
 end.
 
 Ltac solve_opsem :=
-  apply OpsemProps.sInsn__implies__sop_star; 
+  apply OpsemProps.sInsn__implies__sop_plus; 
   econstructor; try solve [
     eauto |
     match goal with
@@ -3128,7 +3359,7 @@ Lemma phinodes_placement_is_correct__dsAlloca: forall (maxb: Values.block)
   (H0 : Opsem.getOperandValue TD v lc gl = ret gns)
   (H1 : gn @ gns) (H2 : malloc TD Mem tsz gn align0 = ret (Mem', mb)),
   exists St1' : Opsem.State,
-     Opsem.sop_star Cfg1 St1 St1' E0 /\
+     Opsem.sop_plus Cfg1 St1 St1' E0 /\
      State_simulation pinfo Cfg1 St1' Cfg2
        {|
        Opsem.ECS := {|
@@ -3173,7 +3404,7 @@ Lemma phinodes_placement_is_correct__dsMalloc: forall (maxb: Values.block)
   (H0 : Opsem.getOperandValue TD v lc gl = ret gns)
   (H1 : gn @ gns) (H2 : malloc TD Mem tsz gn align0 = ret (Mem', mb)),
   exists St1' : Opsem.State,
-     Opsem.sop_star Cfg1 St1 St1' E0 /\
+     Opsem.sop_plus Cfg1 St1 St1' E0 /\
      State_simulation pinfo Cfg1 St1' Cfg2
        {|
        Opsem.ECS := {|
@@ -3425,7 +3656,7 @@ Lemma phinodes_placement_is_correct__dsCall: forall (maxb : Values.block)
   (H3 : Opsem.params2GVs TD lp lc gl = ret gvs)
   (H4 : Opsem.initLocals TD la gvs = ret lc'),
   exists St1' : Opsem.State,
-     Opsem.sop_star Cfg1 St1 St1' E0 /\
+     Opsem.sop_plus Cfg1 St1 St1' E0 /\
      State_simulation pinfo Cfg1 St1' Cfg2
        {|
        Opsem.ECS := {|
@@ -3496,7 +3727,7 @@ Proof.
          ::ECs1) Mem).
     split.
     SSCase "opsem".
-      apply OpsemProps.sInsn__implies__sop_star. 
+      apply OpsemProps.sInsn__implies__sop_plus. 
       econstructor; eauto.
 
     SSCase "sim".
@@ -3555,7 +3786,7 @@ Proof.
          ::ECs1) Mem).
     split.
     SSCase "opsem".
-      apply OpsemProps.sInsn__implies__sop_star. 
+      apply OpsemProps.sInsn__implies__sop_plus. 
       econstructor; eauto.
 
     SSCase "sim".
@@ -3699,7 +3930,7 @@ Lemma phinodes_placement_is_correct__dsExCall: forall (maxb : Values.block)
           ret (oresult, tr, Mem'))
   (H5 : Opsem.exCallUpdateLocals TD ft noret0 rid oresult lc = ret lc'),
   exists St1' : Opsem.State,
-     Opsem.sop_star Cfg1 St1 St1' tr /\
+     Opsem.sop_plus Cfg1 St1 St1' tr /\
      State_simulation pinfo Cfg1 St1' Cfg2       
        {|
        Opsem.ECS := {|
@@ -3740,7 +3971,7 @@ Proof.
       eapply lookupExFdecViaPtr__simulation with (TD:=(los,nts))(gl:=gl)
         (lc1:=lc1)(lc2:=lc) in H1; eauto.
       destruct H1 as [J3 J4].
-      apply OpsemProps.sInsn__implies__sop_star.
+      apply OpsemProps.sInsn__implies__sop_plus.
       econstructor; eauto.
         erewrite params2GVs__simulation with (lc2:=lc); eauto.
           eapply WF_PhiInfo_spec12; eauto.
@@ -3779,7 +4010,7 @@ Proof.
       eapply lookupExFdecViaPtr__simulation with (TD:=(los,nts))(gl:=gl)
         (lc1:=lc1)(lc2:=lc) in H1; eauto.
       destruct H1 as [J3 J4].
-      apply OpsemProps.sInsn__implies__sop_star.
+      apply OpsemProps.sInsn__implies__sop_plus.
       econstructor; eauto.
         erewrite params2GVs__simulation with (lc2:=lc); eauto.
           destruct (fdef_dec (PI_f pinfo) F1); subst; auto; try congruence.
@@ -3797,9 +4028,13 @@ Lemma phinodes_placement_is_bsim : forall maxb pinfo Cfg1 St1 Cfg2 St2 St2' tr
   (Hnoalias: Promotability.wf_State maxb pinfo Cfg1 St1) 
   (Hsim: State_simulation pinfo Cfg1 St1 Cfg2 St2)
   (Hop: Opsem.sInsn Cfg2 St2 St2' tr), 
-  exists St1',
+  (exists St1',
+    Opsem.sop_plus Cfg1 St1 St1' tr /\    
+    State_simulation pinfo Cfg1 St1' Cfg2 St2') \/
+  (exists St1',
     Opsem.sop_star Cfg1 St1 St1' tr /\    
-    State_simulation pinfo Cfg1 St1' Cfg2 St2'.
+    lt (measure St2') (measure St2) /\
+    State_simulation pinfo Cfg1 St1' Cfg2 St2').
 Proof.
   intros.
   (sInsn_cases (induction Hop) Case); 
@@ -3825,11 +4060,12 @@ Focus.
       simpl; try solve [auto | solve_tmnInFdefBlockB].
   eapply returnUpdateLocals_rsim in H1; eauto.
   destruct H1 as [lc1'' [H1 Hrsim'']].
+  left.
   exists 
     (Opsem.mkState ((Opsem.mkEC F1' B1' cs1'0 tmn' lc1'' als')::ECs1) Mem').
   split.
     rewrite <- (@E0_right E0).
-    apply OpsemProps.sInsn__implies__sop_star.
+    apply OpsemProps.sInsn__implies__sop_plus.
     constructor; auto.
   
     repeat (split; eauto 2 using cmds_at_block_tail_next).
@@ -3849,11 +4085,12 @@ Focus.
       simpl; auto
     ].
   destruct Htcmds' as [cs1'0 [EQ Htcmds']]; subst.
+  left.
   exists 
     (Opsem.mkState ((Opsem.mkEC F1' B1' cs1'0 tmn' lc1' als')::ECs1) Mem').
   split.
     rewrite <- (@E0_right E0).
-    apply OpsemProps.sInsn__implies__sop_star.
+    apply OpsemProps.sInsn__implies__sop_plus.
     constructor; auto.
   
     repeat (split; eauto 2 using cmds_at_block_tail_next).
@@ -3863,27 +4100,51 @@ Focus.
       eapply ECs_simulation_tail_stable; eauto.
 Unfocus.
 
-Case "sBranch". eapply phinodes_placement_is_correct__dsBranch; eauto.
+Case "sBranch". 
+  abstract (left; eapply phinodes_placement_is_correct__dsBranch; eauto).
 Case "sBranch_uncond". 
-  eapply phinodes_placement_is_correct__dsBranch_uncond; eauto. 
-Case "sBop". abstract phinodes_placement_is_correct__common.
-Case "sFBop". abstract phinodes_placement_is_correct__common.
-Case "sExtractValue". abstract phinodes_placement_is_correct__common.
-Case "sInsertValue". abstract phinodes_placement_is_correct__common.
-Case "sMalloc". abstract phinodes_placement_is_correct__common.
-Case "sFree". abstract phinodes_placement_is_correct__common.
-Case "sAlloca". abstract phinodes_placement_is_correct__common.
-Case "sLoad". eapply phinodes_placement_is_correct__dsLoad; eauto.
-Case "sStore". eapply phinodes_placement_is_correct__dsStore; eauto.
-Case "sGEP". abstract phinodes_placement_is_correct__common.
-Case "sTrunc". abstract phinodes_placement_is_correct__common.
-Case "sExt". abstract phinodes_placement_is_correct__common.
-Case "sCast". abstract phinodes_placement_is_correct__common.
-Case "sIcmp". abstract phinodes_placement_is_correct__common.
-Case "sFcmp". abstract phinodes_placement_is_correct__common.
-Case "sSelect". abstract phinodes_placement_is_correct__common.
-Case "sCall". eapply phinodes_placement_is_correct__dsCall; eauto.
-Case "sExCall". eapply phinodes_placement_is_correct__dsExCall; eauto.
+  abstract (left; eapply phinodes_placement_is_correct__dsBranch_uncond; eauto). 
+Case "sBop". abstract (left; phinodes_placement_is_correct__common).
+Case "sFBop". abstract (left; phinodes_placement_is_correct__common).
+Case "sExtractValue". abstract (left; phinodes_placement_is_correct__common).
+Case "sInsertValue". abstract (left; phinodes_placement_is_correct__common).
+Case "sMalloc". abstract (left; phinodes_placement_is_correct__common).
+Case "sFree". abstract (left; phinodes_placement_is_correct__common).
+Case "sAlloca". abstract (left; phinodes_placement_is_correct__common).
+Case "sLoad". abstract (eapply phinodes_placement_is_correct__dsLoad; eauto).
+Case "sStore". abstract (eapply phinodes_placement_is_correct__dsStore; eauto).
+Case "sGEP". abstract (left; phinodes_placement_is_correct__common).
+Case "sTrunc". abstract (left; phinodes_placement_is_correct__common).
+Case "sExt". abstract (left; phinodes_placement_is_correct__common).
+Case "sCast". abstract (left; phinodes_placement_is_correct__common).
+Case "sIcmp". abstract (left; phinodes_placement_is_correct__common).
+Case "sFcmp". abstract (left; phinodes_placement_is_correct__common).
+Case "sSelect". abstract (left; phinodes_placement_is_correct__common).
+Case "sCall". 
+  abstract (left; eapply phinodes_placement_is_correct__dsCall; eauto).
+Case "sExCall". 
+  abstract (left; eapply phinodes_placement_is_correct__dsExCall; eauto).
+Qed.
+
+Lemma phinodes_placement_is_bsim' : forall maxb pinfo Cfg1 St1 Cfg2 St2 St2' tr
+  (Hwfpi: WF_PhiInfo pinfo) 
+  (Hwfpp: OpsemPP.wf_State Cfg1 St1) 
+  (Hnoalias: Promotability.wf_State maxb pinfo Cfg1 St1) 
+  (Hsim: State_simulation pinfo Cfg1 St1 Cfg2 St2)
+  (Hop: Opsem.sInsn Cfg2 St2 St2' tr), 
+  exists St1',
+    Opsem.sop_star Cfg1 St1 St1' tr /\    
+    State_simulation pinfo Cfg1 St1' Cfg2 St2'.
+Proof.
+  intros.
+  eapply phinodes_placement_is_bsim in Hsim; eauto.
+  destruct Hsim as [[St1' [J1 J2]] | [St1' [J1 [J2 J3]]]].
+  exists St1'.
+    split; auto.
+      apply OpsemProps.sop_plus__implies__sop_star; auto.
+
+    exists St1'.
+    split; auto.
 Qed.
 
 Ltac destruct_match :=
@@ -4327,6 +4588,7 @@ Proof.
     assumption.
 Qed.
 
+(* Should go to opsem_wf *)
 Lemma preservation_star: forall cfg IS IS' tr (Hwfcfg: OpsemPP.wf_Config cfg),
   @OpsemPP.wf_State DGVs cfg IS ->
   Opsem.sop_star cfg IS IS' tr ->
@@ -4337,89 +4599,90 @@ Proof.
     apply OpsemPP.preservation in H0; auto.
 Qed.  
 
-Lemma promotability_preservation_star: forall cfg IS IS' tr pinfo maxb
-  (Hwfpi: WF_PhiInfo pinfo) (Hwfcfg: OpsemPP.wf_Config cfg)  
-  (Hwfpp: OpsemPP.wf_State cfg IS) 
-  (Hwfg: MemProps.wf_globals maxb (OpsemAux.Globals cfg)) (Hinbd: 0 <= maxb),
-  Promotability.wf_State maxb pinfo cfg IS ->
-  Opsem.sop_star cfg IS IS' tr ->
-  Promotability.wf_State maxb pinfo cfg IS'.
+(* Should go to opsem_wf *)
+Lemma preservation_plus: forall cfg IS IS' tr (Hwfcfg: OpsemPP.wf_Config cfg),
+  @OpsemPP.wf_State DGVs cfg IS ->
+  Opsem.sop_plus cfg IS IS' tr ->
+  OpsemPP.wf_State cfg IS'.
 Proof.
   intros.
-  induction H0; auto.
-    apply IHsop_star.
-      apply OpsemPP.preservation in H0; auto.
-      eapply Promotability.preservation in H0; eauto.
+  apply OpsemProps.sop_plus__implies__sop_star in H0.
+  eapply preservation_star; eauto.
 Qed.  
 
-Lemma sop_star__phiplacement_State_simulation: 
-  forall pinfo cfg1 IS1 cfg2 IS2 tr FS2 maxb
-  (Hwfpi: WF_PhiInfo pinfo) (Hwfcfg: OpsemPP.wf_Config cfg1) 
-  (Hwfpp: OpsemPP.wf_State cfg1 IS1) 
+Section TOPSIM.
+
+Variables (pinfo:PhiInfo) (cfg1:OpsemAux.Config) (IS1:@Opsem.State DGVs) 
+          (cfg2:OpsemAux.Config) (IS2:@Opsem.State DGVs) 
+          (maxb:Values.block).
+
+Hypothesis (Hwfpi: WF_PhiInfo pinfo) 
+  (Hwfcfg: OpsemPP.wf_Config cfg1) (Hwfpp: OpsemPP.wf_State cfg1 IS1) 
   (Hnoalias: Promotability.wf_State maxb pinfo cfg1 IS1)
   (Hwfg: MemProps.wf_globals maxb (OpsemAux.Globals cfg1)) (Hinbd: 0 <= maxb)
-  (Hstsim : State_simulation pinfo cfg1 IS1 cfg2 IS2)
-  (Hopstar : Opsem.sop_star cfg2 IS2 FS2 tr),
+  (Hstsim : State_simulation pinfo cfg1 IS1 cfg2 IS2).
+
+Lemma sop_star__phiplacement_State_simulation: 
+  forall FS2 tr (Hopstar : Opsem.sop_star cfg2 IS2 FS2 tr),
   exists FS1, Opsem.sop_star cfg1 IS1 FS1 tr /\ 
     State_simulation pinfo cfg1 FS1 cfg2 FS2.
 Proof.
   intros.
-  generalize dependent IS1.
+  generalize dependent IS1. clear dependent IS1.
   induction Hopstar; intros.
     exists IS1. split; auto.
 
-    eapply phinodes_placement_is_bsim with (St2':=state2) in Hstsim; eauto.
-    destruct Hstsim as [IS1' [Hopstar' Hstsim]].
-    assert (OpsemPP.wf_Config cfg1 /\ OpsemPP.wf_State cfg1 IS1') as Hwfpp'.
+    eapply phinodes_placement_is_bsim' with (St2':=state2) in Hstsim; eauto.
+    destruct Hstsim as [IS1' [Hopstar' Hstsim']].
+    assert (OpsemPP.wf_State cfg1 IS1') as Hwfpp'.
       apply preservation_star in Hopstar'; auto.
     assert (Promotability.wf_State maxb pinfo cfg1 IS1') as Hnoalias'.
-      eapply promotability_preservation_star in Hopstar'; eauto; try tauto.
-    eapply IHHopstar in Hstsim; eauto; try tauto.
-    destruct Hstsim as [FS1 [Hopstar1 Hstsim]].
+      eapply Promotability.preservation_star in Hopstar'; eauto; try tauto.
+    eapply IHHopstar in Hstsim'; eauto; try tauto.
+    destruct Hstsim' as [FS1 [Hopstar1 Hstsim']].
     exists FS1.
     split; eauto.
       eapply OpsemProps.sop_star_trans; eauto.
 Qed.
 
-Lemma sop_plus__phiplacement_State_simulation: 
-  forall pinfo cfg1 IS1 cfg2 IS2 tr FS2 maxb
-  (Hwfpi: WF_PhiInfo pinfo) (Hwfcfg: OpsemPP.wf_Config cfg1) 
-  (Hwfpp: OpsemPP.wf_State cfg1 IS1) 
-  (Hnoalias: Promotability.wf_State maxb pinfo cfg1 IS1)
-  (Hwfg: MemProps.wf_globals maxb (OpsemAux.Globals cfg1)) (Hinbd: 0 <= maxb)
-  (Hstsim : State_simulation pinfo cfg1 IS1 cfg2 IS2)
-  (Hopplus : Opsem.sop_plus cfg2 IS2 FS2 tr),
-  exists FS1, Opsem.sop_star cfg1 IS1 FS1 tr /\ 
-    State_simulation pinfo cfg1 FS1 cfg2 FS2.
+Lemma sop_div'__phiplacement_State_simulation__sop_wf_div: forall
+  tr (Hdiv : sop_diverges' cfg2 IS2 tr),
+  sop_wf_diverges nat lt cfg1 (measure IS2) IS1 tr.
 Proof.
-  intros.
-  inv Hopplus.
-  eapply phinodes_placement_is_bsim with (St2':=state2) in Hstsim; eauto.
-  destruct Hstsim as [IS1' [Hopstar' Hstsim]].
-  assert (OpsemPP.wf_Config cfg1 /\ OpsemPP.wf_State cfg1 IS1') as Hwfpp'.
-    eapply preservation_star in Hopstar'; eauto.
-  assert (Promotability.wf_State maxb pinfo cfg1 IS1') as Hnoalias'.
-    eapply promotability_preservation_star in Hopstar'; eauto; try tauto.
-  eapply sop_star__phiplacement_State_simulation in Hstsim; eauto; try tauto.
-  destruct Hstsim as [FS1' [Hopstar'' Hstsim]].
-  exists FS1'.
-  split; auto.
-    eapply OpsemProps.sop_star_trans; eauto.
-Qed.
-
-Lemma sop_div__phiplacement_State_simulation: forall pinfo cfg1 IS1 cfg2 IS2 tr 
-  maxb (Hwfpi: WF_PhiInfo pinfo) (Hwfpp: OpsemPP.wf_State cfg1 IS1) 
-  (Hnoalias: Promotability.wf_State maxb pinfo cfg1 IS1)
-  (Hwfg: MemProps.wf_globals maxb (OpsemAux.Globals cfg1)) (Hinbd: 0 <= maxb)
-  (Hstsim : State_simulation pinfo cfg1 IS1 cfg2 IS2)
-  (Hdiv : Opsem.sop_diverges cfg2 IS2 tr),
-  Opsem.sop_diverges cfg1 IS1 tr.
-Proof.
+  repeat match goal with
+  | H:_ |- _ => generalize dependent H; clear H
+  end. 
   cofix CIH.
   intros.
   inv Hdiv.
+  eapply phinodes_placement_is_bsim with (St2':=state2) in Hstsim; eauto.
+  destruct Hstsim as [[St1' [J1 J2]] | [St1' [J1 [J2 J3]]]].    
+    assert (OpsemPP.wf_State cfg1 St1') as Hwfpp'.
+      apply preservation_plus in J1; auto.
+    assert (Promotability.wf_State maxb pinfo cfg1 St1') as Hnoalias'.
+      eapply Promotability.preservation_plus in J1; eauto; try tauto.
+    eapply CIH in J2; eauto; try tauto.
+    eapply sop_wf_diverges_plus; eauto.
 
-Admitted.
+    assert (OpsemPP.wf_State cfg1 St1') as Hwfpp'.
+      apply preservation_star in J1; auto.
+    assert (Promotability.wf_State maxb pinfo cfg1 St1') as Hnoalias'.
+      eapply Promotability.preservation_star in J1; eauto; try tauto.
+    eapply CIH in J3; eauto; try tauto.
+    eapply sop_wf_diverges_star with (m2:=measure state2); eauto.
+Qed.
+
+Lemma sop_div__phiplacement_State_simulation: forall 
+  tr (Hdiv : Opsem.sop_diverges cfg2 IS2 tr),
+  Opsem.sop_diverges cfg1 IS1 tr.
+Proof.
+  intros.
+  apply sop_diverges__sop_diverges' in Hdiv.
+  eapply sop_div'__phiplacement_State_simulation__sop_wf_div in Hdiv; eauto.
+  eapply sop_wf_diverges__sop_diverges; eauto using lt_wf.
+Qed.
+
+End TOPSIM.
 
 Lemma getProductsIDs_app : forall ps1 ps2,
   getProductsIDs (ps1++ps2) = getProductsIDs ps1++getProductsIDs ps2.
@@ -4532,14 +4795,14 @@ Proof.
     inv Hdiv.
     eapply s_genInitState__phiplacement_State_simulation in H; eauto.
     destruct H as [cfg1 [IS1 [Hinit Hstsim]]].  
-    assert (OpsemPP.wf_State cfg1 IS1) as Hwfst. 
+    assert (OpsemPP.wf_Config cfg1 /\ OpsemPP.wf_State cfg1 IS1) as Hwfst. 
       eapply s_genInitState__opsem_wf; eauto.
     assert (exists maxb, 
               MemProps.wf_globals maxb (OpsemAux.Globals cfg1) /\ 0 <= maxb /\
               Promotability.wf_State maxb pinfo cfg1 IS1).
       eapply s_genInitState__wf_globals_promotable; eauto.
     destruct H as [maxb [Hwfg [Hless Hprom]]].
-    eapply sop_div__phiplacement_State_simulation in Hstsim; eauto.
+    eapply sop_div__phiplacement_State_simulation in Hstsim; eauto; try tauto.
     destruct Hstsim as [FS1 Hopdiv1].
     econstructor; eauto.
 Qed.
